bft_qc.v
@@ -1,0 +1,67 @@
+
+Require Import bft2.
+
+Require Import Arith Bool List ZArith. Import ListNotations.
+From QuickChick Require Import QuickChick. Import QcNotation.
+
+(* Suppress some annoying warnings: *)
+Set Warnings "-extraction-opaque-accessed,-extraction".
+
+Require Export ExtLib.Structures.Monads.
+Export MonadNotation. Open Scope monad_scope.
+
+Require Import String. Local Open Scope string.
+
+
+Instance showReplica : Show Replica :=
+{
+  show := fun r:Replica => 
+            match r with
+            | NFReplica id => "NF_" ++ id
+            | FaultyReplica id => "F_" ++ id
+            end
+}.
+
+Definition F := 2.
+Definition SystemSize := 3*F+1.
+Definition NofNFReplicas := 2*F+1.
+
+Definition genFaultyReplica (id : nat) : G Replica :=
+  elems [(FaultyReplica (show id))].
+
+Definition genNFReplica (id : nat) : G Replica :=
+  elems [(NFReplica (show id))].
+
+Fixpoint genSystemSized (sz : nat) (nOf_nfr nOf_f : nat) : G (System) :=
+  match sz with
+    | O => ret [] 
+    | S sz' =>
+        if nOf_f =? F then 
+          (liftM2 cons (genNFReplica sz') (genSystemSized sz' (S nOf_nfr) nOf_f)) 
+        else
+          if nOf_nfr =? NofNFReplicas then
+            (liftM2 cons (genFaultyReplica sz') (genSystemSized sz' nOf_nfr (S nOf_f)))
+          else
+          oneOf [ (liftM2 cons (genNFReplica sz') (genSystemSized sz' (S nOf_nfr) nOf_f)) ;
+                 (liftM2 cons (genFaultyReplica sz') (genSystemSized sz' nOf_nfr (S nOf_f)))
+               ]
+  end.
+
+Sample (genSystemSized SystemSize 0 0).
+
+Definition CorrectSystem (sys:System) := 
+    andb (count_system sys =? 3*F+1) (countNFR_system sys =? 2*F+1).
+
+QuickChick ( forAll (genSystemSized SystemSize 0 0) CorrectSystem ).
+
+Definition CorrectInitState (sys:System) := 
+  CorrectSystem sys ==>
+    let st := initState sys in
+      andb (count_state st =? 3*F+1) (countNFR_state st =? 2*F+1).
+
+QuickChick ( forAll (genSystemSized SystemSize 0 0) CorrectInitState).
+
+Conjecture CountSize_Consistent : forall (sys:System),
+  (count_system sys) = count_state (ReplicateRequest sys (prePrep sys) (initState sys)).
+
+QuickChick CountSize_Consistent.
